bin/Util.ml
@@ -2,4 +2,5 @@ let lst_to_string lst = String.of_seq (List.to_seq lst)
 let string_to_lst s = List.of_seq (String.to_seq s)
 
 let colon_sep fmt () = Format.fprintf fmt ";@ "
+let comma_sep fmt () = Format.fprintf fmt ";@ "
 let newline_sep fmt () = Format.fprintf fmt "@."
